Cleanup and proof scafolding.

proof/invariant-abstract/ARM_HYP/ArchVCPU_AI.thy
@@ -13,64 +13,212 @@ The main theorem
 *)
 
 theory ArchVCPU_AI
-imports "AInvs"
+imports AInvs.ArchDetSchedSchedule_AI
 begin
+
+(* FIXME MOVE *)
+lemma is_tcb_TCB[simp]:
+  "is_tcb (TCB x)"
+ by (simp add: is_tcb_def)
+
+context Arch begin global_naming ARM_A
 
 text {* The top-level invariance *}
 
-definition "cur_vcpu_to_tcb_vcpu cur_vcpu = 
-  (case cur_vcpu of
-   Some (vcpu, True) \<Rightarrow> Some vcpu
-  | _ \<Rightarrow> None)"
+definition
+  "cur_vcpu_to_tcb_vcpu cur_vcpu =
+    (case cur_vcpu of
+       Some (vcpu, True) \<Rightarrow> Some vcpu
+    | _ \<Rightarrow> None)"
+
+(*
 
 lemma get_tcb_ex_invs:
   "invs s \<Longrightarrow> \<exists>tcb. get_tcb (cur_thread s) s = Some tcb"
  by (drule tcb_at_invs, simp add: tcb_at_def)
 
+lemmas cur_tcb_tcb = cur_tcb_def[simplified atomize_eq, THEN iffD1, THEN tcb_at_ko_at]
+
 definition
-  arch_vcpu_tcb_valid :: "'z::state_ext state \<Rightarrow> bool" where  
+  arch_vcpu_tcb_valid :: "'z::state_ext state \<Rightarrow> bool" where
   "arch_vcpu_tcb_valid  s \<equiv>
-    ARM_A.tcb_vcpu (tcb_arch (the (get_tcb (cur_thread s) s))) = cur_vcpu_to_tcb_vcpu (ARM_A.arm_current_vcpu (arch_state s))"
+    ARM_A.tcb_vcpu (tcb_arch (the (get_tcb (cur_thread s) s)))
+       = cur_vcpu_to_tcb_vcpu (ARM_A.arm_current_vcpu (arch_state s))"
+
+lemma "\<forall>tcb. ko_at (TCB tcb) (cur_thread s) \<longrightarrow> P tcb
+
+ obj_at (\<lambda>obj. \<exists>t. obj = TCB t \<longrightarrow>
+                       ARM_A.tcb_vcpu (tcb_arch t) = cur_vcpu_to_tcb_vcpu (ARM_A.arm_current_vcpu (arch_state s))
+                      ) (cur_thread s) s"
+
+
+lemma "obj_at (\<lambda>obj. \<exists>t. obj = TCB t \<longrightarrow>
+                       ARM_A.tcb_vcpu (tcb_arch t) = cur_vcpu_to_tcb_vcpu (ARM_A.arm_current_vcpu (arch_state s))
+                      ) (cur_thread s) s"
+*)
+definition
+  arch_vcpu_tcb_valid_obj :: "arch_state \<Rightarrow> kernel_object \<Rightarrow> bool" where
+  "arch_vcpu_tcb_valid_obj as obj \<equiv>
+     \<forall>t. obj = TCB t \<longrightarrow>
+           ARM_A.tcb_vcpu (tcb_arch t) = cur_vcpu_to_tcb_vcpu (ARM_A.arm_current_vcpu as)"
+
+
+definition
+  arch_vcpu_tcb_valid :: "'z::state_ext state \<Rightarrow> bool" where
+  "arch_vcpu_tcb_valid s \<equiv>
+    obj_at (arch_vcpu_tcb_valid_obj (arch_state s)) (cur_thread s) s"
+
+lemmas arch_vcpu_tcb_valid_kheap_unfold =
+         arch_vcpu_tcb_valid_def
+         arch_vcpu_tcb_valid_obj_def
+         obj_at_def
+         get_tcb_ko_at
 
 lemma arch_vcpu_tcb_valid_trans_st[simp]:
  "arch_vcpu_tcb_valid (trans_state f s) = arch_vcpu_tcb_valid s"
- by (simp add: trans_state_def arch_vcpu_tcb_valid_def get_tcb_def)
+ "arch_vcpu_tcb_valid (trans_state f s\<lparr>cur_thread := cur\<rparr>) = arch_vcpu_tcb_valid (s\<lparr>cur_thread := cur\<rparr>)"
+ by (simp add: trans_state_def arch_vcpu_tcb_valid_def obj_at_def cur_tcb_def)+
 
-lemma arch_vcpu_tcb_valid_set_obj_not_cur_thread:
-  "\<lbrace>arch_vcpu_tcb_valid and (op \<noteq> addr) o cur_thread\<rbrace> set_object addr obj \<lbrace>\<lambda>_. arch_vcpu_tcb_valid\<rbrace>"
-  unfolding set_object_def 
-  apply wpsimp
-  unfolding arch_vcpu_tcb_valid_def get_tcb_def
-  apply simp
+lemma arch_vcpu_tcb_validE:
+  "\<lbrakk> arch_vcpu_tcb_valid s ;
+     arch_state s = arch_state t ;
+     kheap s (cur_thread s) = kheap t (cur_thread t) \<rbrakk>
+   \<Longrightarrow> arch_vcpu_tcb_valid t"
+  apply (clarsimp simp: arch_vcpu_tcb_valid_def obj_at_def cur_tcb_def)
+ done
+
+lemma lift_arch_vcpu_tcb_valid:
+  "\<lbrakk> \<And>P. \<lbrace>\<lambda>s.  P (kheap s (cur_thread s)) \<rbrace> f \<lbrace>\<lambda>_ s.  P (kheap s (cur_thread s))\<rbrace>;
+     \<And>Q. \<lbrace>\<lambda>s.  Q (arch_state s) \<rbrace> f \<lbrace>\<lambda>_ s.  Q (arch_state s)\<rbrace> \<rbrakk>
+ \<Longrightarrow> \<lbrace>arch_vcpu_tcb_valid \<rbrace> f \<lbrace>\<lambda>_. arch_vcpu_tcb_valid\<rbrace>"
+  apply (unfold valid_def)
+  apply clarsimp
+  apply (erule arch_vcpu_tcb_validE)
+   apply (drule_tac x="op = (arch_state s)" in meta_spec)
+   apply fastforce
+  apply (drule_tac x="op = (kheap s (cur_thread s))" in meta_spec)
+  apply fastforce
+ done
+
+
+lemma set_object_not_cur_thread_arch_vcpu_tcb_valid:
+  "\<lbrace>arch_vcpu_tcb_valid and (op \<noteq> addr) \<circ> cur_thread\<rbrace> set_object addr obj \<lbrace>\<lambda>_. arch_vcpu_tcb_valid\<rbrace>"
+  apply (wpsimp simp: set_object_def arch_vcpu_tcb_valid_def)
+  apply (clarsimp simp: cur_tcb_def obj_at_def)
   done
 
-lemma arch_vcpu_tcb_valid_set_obj_cur_thread:
-  "\<lbrace>invs and arch_vcpu_tcb_valid and (op = addr) o cur_thread and (\<lambda>_. is_tcb obj) 
-    and (\<lambda>s. ARM_A.tcb_vcpu (tcb_arch (case obj of TCB tcb \<Rightarrow> tcb)) = cur_vcpu_to_tcb_vcpu (ARM_A.arm_current_vcpu (arch_state s)))
+lemma set_object_cur_thread_arch_vcpu_tcb_valid:
+  "\<lbrace>arch_vcpu_tcb_valid and (op = addr) \<circ> cur_thread and (\<lambda>_. is_tcb obj)
+    and (\<lambda>s. ARM_A.tcb_vcpu (tcb_arch (case obj of TCB tcb \<Rightarrow> tcb))
+               = cur_vcpu_to_tcb_vcpu (ARM_A.arm_current_vcpu (arch_state s)))
     \<rbrace> set_object addr obj \<lbrace>\<lambda>_. arch_vcpu_tcb_valid\<rbrace>"
-  unfolding set_object_def 
-  apply wpsimp
-  unfolding arch_vcpu_tcb_valid_def get_tcb_def
-  apply (case_tac obj; clarsimp simp: is_tcb_def)
+  apply (wpsimp simp: set_object_def arch_vcpu_tcb_valid_def)
+  apply (clarsimp simp: cur_tcb_def obj_at_def arch_vcpu_tcb_valid_obj_def)
   done
+
+lemmas set_object_arch_vcpu_tcb_valid =
+         hoare_pre_disj[OF set_object_not_cur_thread_arch_vcpu_tcb_valid
+                           set_object_cur_thread_arch_vcpu_tcb_valid]
+(*
+thm  ArchVCPU_AI.as_user_arch_vcpu
+ crunch arch_vcpu[wp]:  as_user "arch_vcpu_tcb_valid"
+  (ignore:
+   wp: set_object_arch_vcpu_tcb_valid
+   simp: obj_at_def  arch_vcpu_tcb_valid_def ARM_A.arch_tcb_context_set_def
+   is_tcb_def get_tcb_def)
+thm  ArchVCPU_AI.as_user_arch_vcpu
+*)
+
+lemma as_user_arch_vcpu_tcb_valid[wp]:
+  "\<lbrace>arch_vcpu_tcb_valid \<rbrace> as_user tcb_ptr f \<lbrace>\<lambda>_. arch_vcpu_tcb_valid\<rbrace>"
+  unfolding as_user_def
+  apply (wpsimp wp: set_object_arch_vcpu_tcb_valid)
+  apply (clarsimp simp:  arch_vcpu_tcb_valid_kheap_unfold arch_tcb_context_set_def)
+  done
+
+lemma set_thread_state_arch_vcpu_tcb_valid[wp]:
+ "\<lbrace>arch_vcpu_tcb_valid\<rbrace> set_thread_state ref ts \<lbrace>\<lambda>_. arch_vcpu_tcb_valid\<rbrace>"
+  unfolding set_thread_state_def
+  apply (wpsimp wp: set_object_arch_vcpu_tcb_valid dxo_wp_weak)
+  apply (clarsimp simp: arch_vcpu_tcb_valid_kheap_unfold)
+  done
+
+lemma activate_thread_arch_vcpu_tcb_valid[wp]:
+ "\<lbrace>arch_vcpu_tcb_valid\<rbrace> activate_thread \<lbrace>\<lambda>rv. arch_vcpu_tcb_valid \<rbrace>"
+  unfolding activate_thread_def
+  by (wpsimp wp: gts_wp simp: ARM_A.arch_activate_idle_thread_def)
+
+lemma do_machine_op_arch_vcpu_tcb_valid[wp]:
+  "\<lbrace>\<lambda>s. arch_vcpu_tcb_valid (g s) \<rbrace> do_machine_op f \<lbrace>\<lambda>_ s. arch_vcpu_tcb_valid (g s)\<rbrace>"
+ unfolding do_machine_op_def
+ apply wpsimp
+ apply (clarsimp simp add: cur_tcb_def obj_at_def arch_vcpu_tcb_valid_def)
+apply (rule_tac x=ko in exI)
+
+sorry
+
+lemma vcpu_switch_arch_vcpu_tcb_valid:
+ "\<lbrace>\<lambda>s. arch_vcpu_tcb_valid (s\<lparr>cur_thread := cur\<rparr>)\<rbrace>
+   vcpu_switch (ARM_A.tcb_vcpu (tcb_arch xd))
+  \<lbrace>\<lambda>xa s. arch_vcpu_tcb_valid (s\<lparr>cur_thread := cur\<rparr>)\<rbrace>"
+  apply (clarsimp simp add: vcpu_switch_def split: option.splits)
+  apply (rule conjI; clarsimp)
+  apply (wpsimp simp: ARM_A.vcpu_disable_def)
+sorry
+
+lemma blah:
+  "tcb_at cur s \<Longrightarrow> arch_vcpu_tcb_valid (s\<lparr>cur_thread := cur\<rparr>) \<Longrightarrow> (\<exists>y. get_tcb cur s = Some y) "
+ apply (clarsimp simp add: arch_vcpu_tcb_valid_kheap_unfold is_tcb_def )
+ apply (clarsimp split: kernel_object.splits)
+ done
 
 lemma
- "\<lbrace>invs and arch_vcpu_tcb_valid\<rbrace> activate_thread \<lbrace>\<lambda>rv. arch_vcpu_tcb_valid \<rbrace>"
-unfolding activate_thread_def 
- apply wpsimp
-unfolding set_thread_state_def 
- apply (wpsimp wp: arch_vcpu_tcb_valid_set_obj_cur_thread)
-unfolding as_user_def
- apply (wpsimp wp: arch_vcpu_tcb_valid_set_obj_cur_thread)
+ "\<lbrace>\<lambda>s. (\<exists>y. get_tcb cur s = Some y) \<longrightarrow> arch_vcpu_tcb_valid (s\<lparr>cur_thread := cur\<rparr>)\<rbrace>
+  arm_context_switch x51 x2
+  \<lbrace>\<lambda>xa s. (\<exists>y. get_tcb cur s = Some y) \<longrightarrow> arch_vcpu_tcb_valid (s\<lparr>cur_thread := cur\<rparr>)\<rbrace>"
+  unfolding arm_context_switch_def
+  apply wpsimp
+ oops
+
+lemma set_vm_root_arch_vcpu_tcb_valid:
+  "\<lbrace>\<lambda>s. arch_vcpu_tcb_valid_obj (arch_state s) obj \<and> ko_at obj cur s \<rbrace>
+     set_vm_root cur
+   \<lbrace>\<lambda>x s. arch_vcpu_tcb_valid (s\<lparr>cur_thread := cur\<rparr>)\<rbrace>"
+ unfolding set_vm_root_def
+ apply_trace (wpsimp wp: vcpu_switch_arch_vcpu_tcb_valid)
 oops
 
-lemma schedule_invs:
-  "\<lbrace>invs and (\<lambda>s. e \<noteq> Interrupt \<longrightarrow> ct_running s) and arch_vcpu_tcb_valid \<rbrace>
-  (schedule) :: (unit,unit) s_monad
+lemma arch_switch_to_thread_arch_vcpu_tcb_valid_obj:
+  "\<lbrace>\<lambda>s. arch_vcpu_tcb_valid_obj (arch_state s) obj \<and> ko_at obj cur s \<rbrace>
+      arch_switch_to_thread cur
+   \<lbrace>\<lambda>a s. arch_vcpu_tcb_valid (s\<lparr>cur_thread := cur\<rparr>)\<rbrace>"
+ unfolding arch_switch_to_thread_def
+ apply wpsimp
+ sorry
+
+lemma switch_to_thread_arch_vcpu_tcb_valid:
+ "\<lbrace>\<lambda>s. arch_vcpu_tcb_valid s \<rbrace> switch_to_thread cur \<lbrace>\<lambda>rv. arch_vcpu_tcb_valid\<rbrace>"
+ unfolding switch_to_thread_def
+ apply wpsimp
+ apply (wpsimp wp: dxo_wp_weak assert_wp get_wp arch_switch_to_thread_arch_vcpu_tcb_valid_obj)
+ sorry
+
+lemma switch_to_idle_thread_arch_vcpu_tcb_valid:
+ "\<lbrace>\<lambda>s. arch_vcpu_tcb_valid s \<rbrace> switch_to_idle_thread \<lbrace>\<lambda>rv. arch_vcpu_tcb_valid\<rbrace>"
+sorry
+
+lemma schedule_arch_vcpu_tcb_valid:
+  "\<lbrace>(\<lambda>s. e \<noteq> Interrupt \<longrightarrow> ct_running s) and arch_vcpu_tcb_valid \<rbrace>
+  (schedule) :: (unit, unit) s_monad
   \<lbrace>\<lambda>rv. arch_vcpu_tcb_valid \<rbrace>"
-  unfolding schedule_def 
-using activate_invs
-oops
+  unfolding schedule_def
+  apply (wpsimp wp: alternative_wp dxo_wp_weak assert_wp switch_to_thread_arch_vcpu_tcb_valid )
+  apply (rule lift_arch_vcpu_tcb_valid; wpsimp wp: select_wp)
+  apply (rule lift_arch_vcpu_tcb_valid; wpsimp wp: gets_wp simp: allActiveTCBs_gets)
+  apply (wpsimp wp: gets_wp)
+  apply (wpsimp wp: alternative_wp gets_wp switch_to_idle_thread_arch_vcpu_tcb_valid return_wp)
+  apply (wpsimp wp: )
+done
 (*
 crunch blah[wp]: call_kernel arch_vcpu_tcb_valid
  (simp: get_tcb_ex_invs arch_vcpu_tcb_valid_def)
@@ -79,8 +227,8 @@ theorem akernel_arch_vcpu_tcb_valid_inv:
   "\<lbrace>invs and (\<lambda>s. e \<noteq> Interrupt \<longrightarrow> ct_running s) and arch_vcpu_tcb_valid \<rbrace>
   (call_kernel e) :: (unit,unit) s_monad
   \<lbrace>\<lambda>rv. arch_vcpu_tcb_valid \<rbrace>"
-  unfolding call_kernel_def arch_vcpu_tcb_valid_def
-  apply (wpsimp wp: activate_invs simp: active_from_running get_tcb_ex_invs)
+  unfolding call_kernel_def
+  apply (wpsimp wp: schedule_arch_vcpu_tcb_valid activate_invs simp: active_from_running )
 oops
 
 end
